@prefix : <http://www.semanticweb.org/eleannapanagoulia/ontologies/2020/6/OBPD#> .
@prefix owl: <http://www.w3.org/2002/07/owl#> .
@prefix rdf: <http://www.w3.org/1999/02/22-rdf-syntax-ns#> .
@prefix xml: <http://www.w3.org/XML/1998/namespace> .
@prefix xsd: <http://www.w3.org/2001/XMLSchema#> .
@prefix rdfs: <http://www.w3.org/2000/01/rdf-schema#> .
@base <http://www.semanticweb.org/eleannapanagoulia/ontologies/2020/6/OBPD> .

<http://www.semanticweb.org/eleannapanagoulia/ontologies/2020/6/OBPD> rdf:type owl:Ontology .

#################################################################
#    Object Properties
#################################################################

###  http://www.semanticweb.org/eleannapanagoulia/ontologies/2020/6/OBPD#assignedTo
:assignedTo rdf:type owl:ObjectProperty ;
            owl:inverseOf :referencedFrom ;
            rdfs:domain :MaterialAssembly ,
                        :Program ,
                        :Schedule ,
                        :System ;
            rdfs:range :Zone ,
                       owl:Thing ;
            rdfs:comment "The relationship in which a subject is designated to an object." .


###  http://www.semanticweb.org/eleannapanagoulia/ontologies/2020/6/OBPD#has
:has rdf:type owl:ObjectProperty ;
     rdfs:comment "A relationship between two objects in which the subject can be said to be closely associated with, contain, or can be said to be comprised of another entity." .


###  http://www.semanticweb.org/eleannapanagoulia/ontologies/2020/6/OBPD#hasAnalyticalRepresentation
:hasAnalyticalRepresentation rdf:type owl:ObjectProperty ;
                             rdfs:subPropertyOf :has ;
                             rdfs:domain :Material ,
                                         :Program ,
                                         :System ,
                                         :Zone ;
                             rdfs:range :EnergyPlusBuildingProgram ,
                                        :EnergyPlusMaterial ,
                                        :EnergyPlusSpaceProgram ,
                                        :EnergyPlusZone ,
                                        :RadianceMaterial ;
                             owl:propertyDisjointWith :hasMaterial ;
                             rdfs:comment "Representations of specific data for the purposes of analysis or an analytical environment. For example a material may be represented, for analysis, as defined by Energy Plus or Radiance eqch requiring data to be represented in a different fashion." .


###  http://www.semanticweb.org/eleannapanagoulia/ontologies/2020/6/OBPD#hasMaterial
:hasMaterial rdf:type owl:ObjectProperty ;
             rdfs:subPropertyOf :has ;
             rdfs:domain :Material ;
             rdfs:range :MaterialAssembly ;
             rdfs:comment "A special case of the 'has' property that singifies than an object has a material." .


###  http://www.semanticweb.org/eleannapanagoulia/ontologies/2020/6/OBPD#isAdjacent
:isAdjacent rdf:type owl:ObjectProperty ,
                     owl:SymmetricProperty ;
            rdfs:domain :MaterialAssembly ,
                        :Zone ;
            rdfs:range :MaterialAssembly ,
                       :Zone ;
            rdfs:comment "A topological relationship between two objects (e.g., material layers, zones) that share a common border or boundary, but do not intersect." .


###  http://www.semanticweb.org/eleannapanagoulia/ontologies/2020/6/OBPD#referencedFrom
:referencedFrom rdf:type owl:ObjectProperty ;
                rdfs:comment "(Inverse of assignedTo)" .


#################################################################
#    Data properties
#################################################################

###  http://www.semanticweb.org/eleannapanagoulia/ontologies/2020/6/OBPD#area
:area rdf:type owl:DatatypeProperty ;
      rdfs:subPropertyOf :metric ;
      rdf:type owl:FunctionalProperty ;
      rdfs:domain :Zone ;
      rdfs:range xsd:double ;
      owl:propertyDisjointWith :volume ;
      rdfs:comment "The numerical representation of the area of a zone." .


###  http://www.semanticweb.org/eleannapanagoulia/ontologies/2020/6/OBPD#coolingSetpoint
:coolingSetpoint rdf:type owl:DatatypeProperty ;
                 rdfs:subPropertyOf :setpoint ;
                 rdfs:domain :System ;
                 rdfs:range xsd:double ;
                 rdfs:comment "The temperature at which cooling begins." .


###  http://www.semanticweb.org/eleannapanagoulia/ontologies/2020/6/OBPD#coolingSetpointImperial
:coolingSetpointImperial rdf:type owl:DatatypeProperty ;
                         rdfs:subPropertyOf :coolingSetpoint ;
                         rdf:type owl:FunctionalProperty ;
                         rdfs:domain :System ;
                         rdfs:range xsd:double ;
                         owl:propertyDisjointWith :coolingSetpointMetric ;
                         rdfs:comment "The cooling setpoint in degrees fahrenheit (F)." .


###  http://www.semanticweb.org/eleannapanagoulia/ontologies/2020/6/OBPD#coolingSetpointMetric
:coolingSetpointMetric rdf:type owl:DatatypeProperty ;
                       rdfs:subPropertyOf :coolingSetpoint ;
                       rdf:type owl:FunctionalProperty ;
                       rdfs:domain :System ;
                       rdfs:range xsd:double ;
                       rdfs:comment "The cooling setpoint in degrees celsius (c)." .


###  http://www.semanticweb.org/eleannapanagoulia/ontologies/2020/6/OBPD#dehumidificationSetpoint
:dehumidificationSetpoint rdf:type owl:DatatypeProperty ;
                          rdfs:subPropertyOf :setpoint ;
                          rdfs:domain :System ;
                          rdfs:range xsd:double ;
                          rdfs:comment "The relative humidity percentage at which dehumidification begins." .


###  http://www.semanticweb.org/eleannapanagoulia/ontologies/2020/6/OBPD#description
:description rdf:type owl:DatatypeProperty ;
             rdfs:domain :Document ,
                         :Material ,
                         :MaterialAssembly ,
                         :Program ,
                         :Schedule ,
                         :System ,
                         :Zone ;
             rdfs:range xsd:string ;
             rdfs:comment "Data property of type string that describes an object." .


###  http://www.semanticweb.org/eleannapanagoulia/ontologies/2020/6/OBPD#energyPlusMaterialConductivity
:energyPlusMaterialConductivity rdf:type owl:DatatypeProperty ;
                                rdfs:subPropertyOf :energyPlusMaterialProperty ;
                                rdfs:domain :EnergyPlusMaterial ;
                                rdfs:range xsd:double ;
                                rdfs:comment "The amount of energy conducted through a material in W/(m*K)" .


###  http://www.semanticweb.org/eleannapanagoulia/ontologies/2020/6/OBPD#energyPlusMaterialDensity
:energyPlusMaterialDensity rdf:type owl:DatatypeProperty ;
                           rdfs:subPropertyOf :energyPlusMaterialProperty ;
                           rdfs:domain :EnergyPlusMaterial ;
                           rdfs:range xsd:double ;
                           rdfs:comment "The density of a material in kg/m3." .


###  http://www.semanticweb.org/eleannapanagoulia/ontologies/2020/6/OBPD#energyPlusMaterialProperty
:energyPlusMaterialProperty rdf:type owl:DatatypeProperty ;
                            rdfs:subPropertyOf :materialProperty ;
                            rdfs:domain :EnergyPlusMaterial ;
                            rdfs:range xsd:string ;
                            rdfs:comment "This property is used to describe an Energy Plus material. This property may be used to store a full or partial definition as a string that can be later parsed."^^xsd:string .


###  http://www.semanticweb.org/eleannapanagoulia/ontologies/2020/6/OBPD#energyPlusMaterialRValue
:energyPlusMaterialRValue rdf:type owl:DatatypeProperty ;
                          rdfs:subPropertyOf :energyPlusMaterialProperty ;
                          rdfs:domain :EnergyPlusMaterial ;
                          rdfs:range xsd:double ;
                          rdfs:comment "The thermal resistance of a material." .


###  http://www.semanticweb.org/eleannapanagoulia/ontologies/2020/6/OBPD#energyPlusMaterialRoughness
:energyPlusMaterialRoughness rdf:type owl:DatatypeProperty ;
                             rdfs:subPropertyOf :energyPlusMaterialProperty ;
                             rdfs:domain :EnergyPlusMaterial ;
                             rdfs:range xsd:string ;
                             rdfs:comment "This property defines the roughness of a material as defined by the Energy Plus 8.3 input-output documentation." .


###  http://www.semanticweb.org/eleannapanagoulia/ontologies/2020/6/OBPD#energyPlusMaterialSolarAbsorptance
:energyPlusMaterialSolarAbsorptance rdf:type owl:DatatypeProperty ;
                                    rdfs:subPropertyOf :energyPlusMaterialProperty ;
                                    rdfs:domain :EnergyPlusMaterial ;
                                    rdfs:range xsd:double ;
                                    rdfs:comment "The amount of solar energy absorbed by a material." .


###  http://www.semanticweb.org/eleannapanagoulia/ontologies/2020/6/OBPD#energyPlusMaterialSpecificHeat
:energyPlusMaterialSpecificHeat rdf:type owl:DatatypeProperty ;
                                rdfs:subPropertyOf :energyPlusMaterialProperty ;
                                rdfs:domain :EnergyPlusMaterial ;
                                rdfs:range xsd:double ;
                                rdfs:comment "The specific heat of a material in kJ/(kg*K)." .


###  http://www.semanticweb.org/eleannapanagoulia/ontologies/2020/6/OBPD#energyPlusMaterialThermalAbsorptance
:energyPlusMaterialThermalAbsorptance rdf:type owl:DatatypeProperty ;
                                      rdfs:subPropertyOf :energyPlusMaterialProperty ;
                                      rdfs:domain :EnergyPlusMaterial ;
                                      rdfs:range xsd:double ;
                                      rdfs:comment "Amount of heat absorbed by a material in W/m2." .


###  http://www.semanticweb.org/eleannapanagoulia/ontologies/2020/6/OBPD#energyPlusMaterialThermalCapacity
:energyPlusMaterialThermalCapacity rdf:type owl:DatatypeProperty ;
                                   rdfs:subPropertyOf :energyPlusMaterialProperty ;
                                   rdfs:domain :EnergyPlusMaterial ;
                                   rdfs:range xsd:double ;
                                   rdfs:comment "The thermal capacity of a material in kJ/(m2*K)." .


###  http://www.semanticweb.org/eleannapanagoulia/ontologies/2020/6/OBPD#energyPlusMaterialThermalMass
:energyPlusMaterialThermalMass rdf:type owl:DatatypeProperty ;
                               rdfs:subPropertyOf :energyPlusMaterialProperty ;
                               rdfs:domain :EnergyPlusMaterial ;
                               rdfs:range xsd:double ;
                               rdfs:comment "The thermal mass of a material in kg/m2." .


###  http://www.semanticweb.org/eleannapanagoulia/ontologies/2020/6/OBPD#energyPlusMaterialThermalResistance
:energyPlusMaterialThermalResistance rdf:type owl:DatatypeProperty ;
                                     rdfs:subPropertyOf :energyPlusMaterialProperty ;
                                     rdfs:domain :EnergyPlusMaterial ;
                                     rdfs:range xsd:double ;
                                     rdfs:comment "The amount of resistance against thermal exchange by the material in (m2*K)/W." .


###  http://www.semanticweb.org/eleannapanagoulia/ontologies/2020/6/OBPD#energyPlusMaterialVisibleAbsorptance
:energyPlusMaterialVisibleAbsorptance rdf:type owl:DatatypeProperty ;
                                      rdfs:subPropertyOf :energyPlusMaterialProperty ;
                                      rdfs:domain :EnergyPlusMaterial ;
                                      rdfs:range xsd:double ;
                                      rdfs:comment "The amount of visible light absorbed by a material for the purposes of energy modeling." .


###  http://www.semanticweb.org/eleannapanagoulia/ontologies/2020/6/OBPD#energyPlusProgramProperty
:energyPlusProgramProperty rdf:type owl:DatatypeProperty ;
                           rdfs:subPropertyOf :programProperty .


###  http://www.semanticweb.org/eleannapanagoulia/ontologies/2020/6/OBPD#equipmentWattsArea
:equipmentWattsArea rdf:type owl:DatatypeProperty ;
                    rdfs:subPropertyOf :energyPlusProgramProperty ;
                    rdf:type owl:FunctionalProperty ;
                    rdfs:domain :EnergyPlusBuildingProgram ,
                                :EnergyPlusSpaceProgram ,
                                :Program ;
                    rdfs:range xsd:double ;
                    rdfs:comment "The number of watts per area for equipment (e.g., computers etc.) used by a specified program in units of W/m2." .


###  http://www.semanticweb.org/eleannapanagoulia/ontologies/2020/6/OBPD#flowRateArea
:flowRateArea rdf:type owl:DatatypeProperty ;
              rdfs:subPropertyOf :rate ;
              rdf:type owl:FunctionalProperty ;
              rdfs:domain :EnergyPlusBuildingProgram ,
                          :EnergyPlusSpaceProgram ,
                          :Program ;
              rdfs:range xsd:double ;
              owl:propertyDisjointWith :infiltrationRate ;
              rdfs:comment "The amount of fresh air that must be supplied for per meter of floor area for a given program in m3/second." .


###  http://www.semanticweb.org/eleannapanagoulia/ontologies/2020/6/OBPD#heatingSetpoint
:heatingSetpoint rdf:type owl:DatatypeProperty ;
                 rdfs:subPropertyOf :setpoint ;
                 rdfs:domain :System ;
                 rdfs:range xsd:double ;
                 rdfs:comment "The setting at which heating begins." .


###  http://www.semanticweb.org/eleannapanagoulia/ontologies/2020/6/OBPD#heatingSetpointImperial
:heatingSetpointImperial rdf:type owl:DatatypeProperty ;
                         rdfs:subPropertyOf :heatingSetpoint ;
                         rdfs:domain :System ;
                         rdfs:range xsd:double ;
                         owl:propertyDisjointWith :heatingSetpointMetric ;
                         rdfs:comment "The heating setpoint in degrees fahrenheit (F)." .


###  http://www.semanticweb.org/eleannapanagoulia/ontologies/2020/6/OBPD#heatingSetpointMetric
:heatingSetpointMetric rdf:type owl:DatatypeProperty ;
                       rdfs:subPropertyOf :heatingSetpoint ;
                       rdfs:domain :System ;
                       rdfs:range xsd:double ;
                       rdfs:comment "The heating setpoint in degress celsius (c)." .


###  http://www.semanticweb.org/eleannapanagoulia/ontologies/2020/6/OBPD#humiditySetPoint
:humiditySetPoint rdf:type owl:DatatypeProperty ;
                  rdfs:subPropertyOf :setpoint ;
                  rdfs:domain :System ;
                  rdfs:range xsd:double ;
                  rdfs:comment "The relative humidity at which the air is humidified." .


###  http://www.semanticweb.org/eleannapanagoulia/ontologies/2020/6/OBPD#infiltrationRate
:infiltrationRate rdf:type owl:DatatypeProperty ;
                  rdfs:subPropertyOf :rate ;
                  rdf:type owl:FunctionalProperty ;
                  rdfs:domain :EnergyPlusBuildingProgram ,
                              :EnergyPlusSpaceProgram ,
                              :Program ;
                  rdfs:range xsd:double ;
                  rdfs:comment "The rate at which air is exchanged through the facade in air exchanges air changes per hour." .


###  http://www.semanticweb.org/eleannapanagoulia/ontologies/2020/6/OBPD#infiltrationRateImperial
:infiltrationRateImperial rdf:type owl:DatatypeProperty ;
                          rdfs:subPropertyOf :infiltrationRate ;
                          rdfs:comment "Imperial representation of the infiltration rate in cubic feet of air per minute (CFM)." .


###  http://www.semanticweb.org/eleannapanagoulia/ontologies/2020/6/OBPD#infiltrationRateMetric
:infiltrationRateMetric rdf:type owl:DatatypeProperty ;
                        rdfs:subPropertyOf :infiltrationRate ;
                        rdfs:domain :EnergyPlusBuildingProgram ,
                                    :EnergyPlusSpaceProgram ,
                                    :Program ;
                        rdfs:range xsd:double ;
                        rdfs:comment "Metric representation of the infiltration rate in litres of air per second (L/s)." .


###  http://www.semanticweb.org/eleannapanagoulia/ontologies/2020/6/OBPD#lightingWattsArea
:lightingWattsArea rdf:type owl:DatatypeProperty ;
                   rdfs:subPropertyOf :energyPlusProgramProperty ;
                   rdf:type owl:FunctionalProperty ;
                   rdfs:domain :EnergyPlusBuildingProgram ,
                               :EnergyPlusSpaceProgram ,
                               :Program ;
                   rdfs:range xsd:double ;
                   rdfs:comment "The amount of energy consumed for lighting for a given program type in W/m2." .


###  http://www.semanticweb.org/eleannapanagoulia/ontologies/2020/6/OBPD#materialEnumeration
:materialEnumeration rdf:type owl:DatatypeProperty ;
                     rdfs:subPropertyOf :materialProperty ;
                     rdfs:domain :Layer ;
                     rdfs:range xsd:integer ;
                     rdfs:comment "Data property of type integer that describes the ordinal position of a layer from exterior to interior. Required: TRUE. Note: Note: Only used for material assembly." .


###  http://www.semanticweb.org/eleannapanagoulia/ontologies/2020/6/OBPD#materialProperty
:materialProperty rdf:type owl:DatatypeProperty ;
                  rdfs:domain :Material ;
                  rdfs:range rdfs:Literal .


###  http://www.semanticweb.org/eleannapanagoulia/ontologies/2020/6/OBPD#materialThickness
:materialThickness rdf:type owl:DatatypeProperty ;
                   rdfs:subPropertyOf :materialProperty ;
                   rdfs:domain :Layer ;
                   rdfs:range xsd:double ;
                   rdfs:comment "Data property of type double that describes the thickness of material layer. Required: TRUE" .


###  http://www.semanticweb.org/eleannapanagoulia/ontologies/2020/6/OBPD#metric
:metric rdf:type owl:DatatypeProperty ;
        rdfs:range xsd:double .


###  http://www.semanticweb.org/eleannapanagoulia/ontologies/2020/6/OBPD#name
:name rdf:type owl:DatatypeProperty ,
               owl:FunctionalProperty ;
      rdfs:domain :Document ,
                  :Material ,
                  :MaterialAssembly ,
                  :Schedule ,
                  :System ,
                  :Zone ;
      rdfs:range xsd:string ;
      rdfs:comment "Data property of type string that defines the name of a level. Required:TRUE." .


###  http://www.semanticweb.org/eleannapanagoulia/ontologies/2020/6/OBPD#programProperty
:programProperty rdf:type owl:DatatypeProperty ;
                 rdfs:domain :Program ;
                 rdfs:range rdfs:Literal .


###  http://www.semanticweb.org/eleannapanagoulia/ontologies/2020/6/OBPD#programType
:programType rdf:type owl:DatatypeProperty ;
             rdfs:subPropertyOf :programProperty ;
             rdf:type owl:FunctionalProperty ;
             rdfs:domain :EnergyPlusBuildingProgram ,
                         :EnergyPlusSpaceProgram ,
                         :Program ;
             rdfs:range xsd:string ;
             rdfs:comment "The type of program being described for either a building or space (i.e, School, Classroom, Kitchen, Hallway, Multifamily Residential etc.)" .


###  http://www.semanticweb.org/eleannapanagoulia/ontologies/2020/6/OBPD#radianceMaterialProperty
:radianceMaterialProperty rdf:type owl:DatatypeProperty ;
                          rdfs:subPropertyOf :materialProperty ;
                          rdfs:domain :Layer ;
                          rdfs:range xsd:string ;
                          rdfs:comment "This property is used to describe an Radiance material. This property may be used to store a full or partial definition as a string that can be later parsed." .


###  http://www.semanticweb.org/eleannapanagoulia/ontologies/2020/6/OBPD#radianceMaterialPropertyBlue
:radianceMaterialPropertyBlue rdf:type owl:DatatypeProperty ;
                              rdfs:subPropertyOf :radianceMaterialProperty ;
                              rdfs:domain :RadianceMaterial ;
                              rdfs:range xsd:integer ;
                              rdfs:comment "The value for the blue channel minimum value 0 maximum value 255" .


###  http://www.semanticweb.org/eleannapanagoulia/ontologies/2020/6/OBPD#radianceMaterialPropertyGreen
:radianceMaterialPropertyGreen rdf:type owl:DatatypeProperty ;
                               rdfs:subPropertyOf :radianceMaterialProperty ;
                               rdfs:domain :RadianceMaterial ;
                               rdfs:range xsd:integer ;
                               rdfs:comment "value for the green channel." .


###  http://www.semanticweb.org/eleannapanagoulia/ontologies/2020/6/OBPD#radianceMaterialPropertyRed
:radianceMaterialPropertyRed rdf:type owl:DatatypeProperty ;
                             rdfs:subPropertyOf :radianceMaterialProperty ;
                             rdfs:comment "Value for the red channel." .


###  http://www.semanticweb.org/eleannapanagoulia/ontologies/2020/6/OBPD#radianceMaterialPropertyReflectivity
:radianceMaterialPropertyReflectivity rdf:type owl:DatatypeProperty ;
                                      rdfs:subPropertyOf :radianceMaterialProperty ;
                                      rdfs:domain :RadianceMaterial ;
                                      rdfs:range xsd:double ;
                                      rdfs:comment "Percentage of visible light reflected by a material." .


###  http://www.semanticweb.org/eleannapanagoulia/ontologies/2020/6/OBPD#radianceMaterialPropertyTransmissivity
:radianceMaterialPropertyTransmissivity rdf:type owl:DatatypeProperty ;
                                        rdfs:subPropertyOf :radianceMaterialProperty ;
                                        rdfs:domain :RadianceMaterial ;
                                        rdfs:range xsd:double ;
                                        rdfs:comment "Percentage of visible light transmitted through a material, as defined in the Radiance documentation." .


###  http://www.semanticweb.org/eleannapanagoulia/ontologies/2020/6/OBPD#rate
:rate rdf:type owl:DatatypeProperty ;
      rdfs:subPropertyOf :programProperty ;
      rdfs:domain :Program ;
      rdfs:range xsd:double .


###  http://www.semanticweb.org/eleannapanagoulia/ontologies/2020/6/OBPD#setpoint
:setpoint rdf:type owl:DatatypeProperty ;
          rdfs:range xsd:double .


###  http://www.semanticweb.org/eleannapanagoulia/ontologies/2020/6/OBPD#volume
:volume rdf:type owl:DatatypeProperty ;
        rdfs:subPropertyOf :metric ;
        rdf:type owl:FunctionalProperty ;
        rdfs:domain :Zone ;
        rdfs:range xsd:double ;
        rdfs:comment "The numerical representation of the volume of air contained within a zone." .


#################################################################
#    Classes
#################################################################

###  http://www.semanticweb.org/eleannapanagoulia/ontologies/2020/6/OBPD#AirGap
:AirGap rdf:type owl:Class ;
        rdfs:subClassOf :EnergyPlusMaterial ;
        rdfs:comment "The class that describes a MaterialAssembly that is of the Energy Plus type AirGap." .


###  http://www.semanticweb.org/eleannapanagoulia/ontologies/2020/6/OBPD#Document
:Document rdf:type owl:Class ;
          rdfs:comment "Base class for all types of documents that are associated wih an analysis process." .


###  http://www.semanticweb.org/eleannapanagoulia/ontologies/2020/6/OBPD#EnergyPlusBuildingProgram
:EnergyPlusBuildingProgram rdf:type owl:Class ;
                           rdfs:subClassOf :Program ;
                           owl:disjointWith :EnergyPlusSpaceProgram ;
                           rdfs:comment "The class that describes the Energy Plus representation of a building program (i.e.,Residential)." .


###  http://www.semanticweb.org/eleannapanagoulia/ontologies/2020/6/OBPD#EnergyPlusMaterial
:EnergyPlusMaterial rdf:type owl:Class ;
                    rdfs:subClassOf :Material ;
                    owl:disjointWith :RadianceMaterial ;
                    rdfs:comment "The class that decribes the EnergyPlus representation of a MaterialAssembly. EnergyPlusMaterial represents the default, preferred material type according to Energy Plus documentation and it requires knowledge of many of the thermal properties of the material." .


###  http://www.semanticweb.org/eleannapanagoulia/ontologies/2020/6/OBPD#EnergyPlusSpaceProgram
:EnergyPlusSpaceProgram rdf:type owl:Class ;
                        rdfs:subClassOf :Program ;
                        rdfs:comment "The class that describes the Energy Plus representation of a space program (i.e., Living Room)." .


###  http://www.semanticweb.org/eleannapanagoulia/ontologies/2020/6/OBPD#EnergyPlusZone
:EnergyPlusZone rdf:type owl:Class ;
                rdfs:subClassOf :Zone ;
                rdfs:comment "The class that describes the Energy Plus representation of a single HVAC zone." .


###  http://www.semanticweb.org/eleannapanagoulia/ontologies/2020/6/OBPD#InfraredTransparent
:InfraredTransparent rdf:type owl:Class ;
                     rdfs:subClassOf :EnergyPlusMaterial ;
                     rdfs:comment "The class that describes a MAterialAssembly that is of the Energy Plus type InfraredTransparent." .


###  http://www.semanticweb.org/eleannapanagoulia/ontologies/2020/6/OBPD#Layer
:Layer rdf:type owl:Class ;
       rdfs:subClassOf :MaterialAssembly ;
       rdfs:comment "The class that describes numerically the physical properties of a material layer that is part of an assembly." .


###  http://www.semanticweb.org/eleannapanagoulia/ontologies/2020/6/OBPD#Material
:Material rdf:type owl:Class ;
          rdfs:comment "The class that describes numerically the physical properties of a material." .


###  http://www.semanticweb.org/eleannapanagoulia/ontologies/2020/6/OBPD#MaterialAssembly
:MaterialAssembly rdf:type owl:Class ;
                  rdfs:comment "The class that describes the way materials are layered. It also contains the physical properties of the assembly." .


###  http://www.semanticweb.org/eleannapanagoulia/ontologies/2020/6/OBPD#NoMass
:NoMass rdf:type owl:Class ;
        rdfs:subClassOf :EnergyPlusMaterial ;
        rdfs:comment "The class that describes a MaterialAssembly that is of the Energy Plus type NoMass." .


###  http://www.semanticweb.org/eleannapanagoulia/ontologies/2020/6/OBPD#Opaque
:Opaque rdf:type owl:Class ;
        rdfs:subClassOf :RadianceMaterial ;
        owl:disjointWith :Translucent ;
        rdfs:comment "The class that describes a MaterialAssembly that is of the Radiance material type Opaque." .


###  http://www.semanticweb.org/eleannapanagoulia/ontologies/2020/6/OBPD#Program
:Program rdf:type owl:Class .


###  http://www.semanticweb.org/eleannapanagoulia/ontologies/2020/6/OBPD#RadianceMaterial
:RadianceMaterial rdf:type owl:Class ;
                  rdfs:subClassOf :Material ;
                  rdfs:comment "The class that decribes the Radiance representation of a MaterialAssembly." .


###  http://www.semanticweb.org/eleannapanagoulia/ontologies/2020/6/OBPD#RoofVegetation
:RoofVegetation rdf:type owl:Class ;
                rdfs:subClassOf :EnergyPlusMaterial ;
                rdfs:comment "The class that describes a MaterialAssembly that is of the Energy Plus type  RoofVegetation." .


###  http://www.semanticweb.org/eleannapanagoulia/ontologies/2020/6/OBPD#Schedule
:Schedule rdf:type owl:Class ;
          rdfs:comment "The class that describes the operation of a single social or mechanical system." .


###  http://www.semanticweb.org/eleannapanagoulia/ontologies/2020/6/OBPD#System
:System rdf:type owl:Class ;
        rdfs:comment "The class that describes the type and operational parameters of a mechanical or nat. vent. system." .


###  http://www.semanticweb.org/eleannapanagoulia/ontologies/2020/6/OBPD#Translucent
:Translucent rdf:type owl:Class ;
             rdfs:subClassOf :RadianceMaterial ;
             rdfs:comment "The class that describes a MaterialAssembly that is of the Radiance material type Translucent." .


###  http://www.semanticweb.org/eleannapanagoulia/ontologies/2020/6/OBPD#Zone
:Zone rdf:type owl:Class ;
      rdfs:comment "The class that describes the operation of an HVAC zone (is conditioned etc.)." .


#################################################################
#    General axioms
#################################################################

[ rdf:type owl:AllDisjointClasses ;
  owl:members ( :AirGap
                :InfraredTransparent
                :NoMass
                :RoofVegetation
              )
] .


[ rdf:type owl:AllDisjointClasses ;
  owl:members ( :Document
                :Material
                :MaterialAssembly
                :Program
                :Schedule
                :System
                :Zone
              )
] .


[ rdf:type owl:AllDisjointProperties ;
  owl:members ( :assignedTo
                :has
                :isAdjacent
                :referencedFrom
              )
] .


[ rdf:type owl:AllDisjointProperties ;
  owl:members ( :coolingSetpoint
                :dehumidificationSetpoint
                :heatingSetpoint
                :humiditySetPoint
              )
] .


[ rdf:type owl:AllDisjointProperties ;
  owl:members ( :description
                :materialProperty
                :metric
                :name
                :programProperty
                :setpoint
              )
] .


[ rdf:type owl:AllDisjointProperties ;
  owl:members ( :energyPlusMaterialConductivity
                :energyPlusMaterialDensity
                :energyPlusMaterialRValue
                :energyPlusMaterialRoughness
                :energyPlusMaterialSolarAbsorptance
                :energyPlusMaterialSpecificHeat
                :energyPlusMaterialThermalAbsorptance
                :energyPlusMaterialThermalCapacity
                :energyPlusMaterialThermalMass
                :energyPlusMaterialThermalResistance
                :energyPlusMaterialVisibleAbsorptance
              )
] .


[ rdf:type owl:AllDisjointProperties ;
  owl:members ( :energyPlusMaterialProperty
                :materialEnumeration
                :materialThickness
                :radianceMaterialProperty
              )
] .


[ rdf:type owl:AllDisjointProperties ;
  owl:members ( :radianceMaterialPropertyBlue
                :radianceMaterialPropertyGreen
                :radianceMaterialPropertyRed
                :radianceMaterialPropertyReflectivity
                :radianceMaterialPropertyTransmissivity
              )
] .


###  Generated by the OWL API (version 4.5.9.2019-02-01T07:24:44Z) https://github.com/owlcs/owlapi
